WIP binencoders

src/BinEncoders/Libraries/Bool.v
@@ -2,7 +2,7 @@ Require Import Fiat.BinEncoders.Specs
                Fiat.BinEncoders.Libraries.BinCore.
 
 Section BoolBinEncoder.
-  Definition Bool_encode (b : bool) : bin_t := b :: nil.
+  Definition Bool_encode_inner (b : bool) : bin_t := b :: nil.
 
   Definition Bool_decode (b : bin_t) : bool * bin_t :=
     match b with
@@ -10,9 +10,16 @@ Section BoolBinEncoder.
     | x :: xs => (x, xs)
     end.
 
-  Theorem Bool_encode_correct : bin_encode_correct Bool_encode Bool_decode.
+  Theorem Bool_encode_correct : bin_encode_correct Bool_encode_inner Bool_decode.
   Proof.
-    unfold bin_encode_correct, Bool_encode, Bool_decode.
+    unfold bin_encode_correct, Bool_encode_inner, Bool_decode.
     eauto.
   Qed.
 End BoolBinEncoder.
+
+Definition Bool_encode :=
+  bin_encode_transform_pair Bool_encode_inner.
+
+Global Instance Bool_decoder
+  : decoder (fun _ => True) Bool_encode :=
+  bin_encode_transform_pair_decoder Bool_encode_correct.
