src/BinEncoders/Libraries/Char.v
@@ -5,8 +5,8 @@ Require Import Coq.omega.Omega
                Fiat.BinEncoders.Libraries.FixInt.
 
 Section CharBinEncoder.
-  Definition Char_encode (c : ascii) : bin_t.
-    refine (@FixInt_encode 8 (exist _ (N_of_ascii c) _)).
+  Definition Char_encode_inner (c : ascii) : bin_t.
+    refine (@FixInt_encode_inner 8 (exist _ (N_of_ascii c) _)).
     unfold exp2; unfold exp2'.
     induction c.
     repeat (match goal with
@@ -18,11 +18,18 @@ Section CharBinEncoder.
     let (n, ext) := FixInt_decode 8 b
     in  (ascii_of_N (proj1_sig n), ext).
 
-  Theorem Char_encode_correct : bin_encode_correct Char_encode Char_decode.
+  Theorem Char_encode_correct : bin_encode_correct Char_encode_inner Char_decode.
   Proof.
-    unfold bin_encode_correct, Char_encode, Char_decode.
+    unfold bin_encode_correct, Char_encode_inner, Char_decode.
     intros c ext.
     rewrite FixInt_encode_correct; simpl.
     rewrite ascii_N_embedding. reflexivity.
   Qed.
 End CharBinEncoder.
+
+Definition Char_encode :=
+  bin_encode_transform_pair Char_encode_inner.
+
+Global Instance Char_decoder
+  : decoder (fun _ => True) Char_encode :=
+  bin_encode_transform_pair_decoder Char_encode_correct.
